proof/invariant-abstract/AARCH64/ArchDetSchedSchedule_AI.thy
@@ -13,32 +13,13 @@ context Arch begin arch_global_naming
 
 named_theorems DetSchedSchedule_AI_assms
 
-crunch
-  prepare_thread_delete
-  for prepare_thread_delete_idle_thread[wp, DetSchedSchedule_AI_assms]: "\<lambda>(s:: det_ext state). P (idle_thread s)"
+crunch prepare_thread_delete
+  for idle_thread[wp, DetSchedSchedule_AI_assms]: "\<lambda>s. P (idle_thread s)"
   (wp: crunch_wps)
 
-crunch set_vcpu
-  for exst[wp]: "\<lambda>s. P (exst s)" (wp: crunch_wps)
-
-crunch vcpu_disable, vcpu_restore, vcpu_save, vcpu_switch
+crunch set_vcpu, vcpu_disable, vcpu_restore, vcpu_save, vcpu_switch, switch_to_idle_thread, set_vm_root
   for exst[wp]: "\<lambda>s. P (exst s)"
   (wp: crunch_wps)
-
-lemma pred_tcb_atP[wp]:
-  "\<lbrace>\<lambda>s. P (pred_tcb_at proj Q t s)\<rbrace> set_vcpu prt vcpu \<lbrace>\<lambda>_ s. P (pred_tcb_at proj Q t s)\<rbrace>"
-  unfolding set_vcpu_def set_object_def
-  apply (wp get_object_wp)
-  apply (clarsimp simp: pred_tcb_at_def obj_at_def split: kernel_object.splits)
-  done
-
-crunch vcpu_disable, vcpu_enable, vcpu_restore, vcpu_save
-  for pred_tcb_atP[wp]: "\<lambda>s. P (pred_tcb_at proj Q t s)"
-  (wp: crunch_wps simp: crunch_simps)
-
-lemma vcpu_switch_pred_tcb_at[wp]:
-  "\<lbrace>\<lambda>s. P (pred_tcb_at proj Q t s)\<rbrace> vcpu_switch vcpu \<lbrace>\<lambda>_ s. P (pred_tcb_at proj Q t s)\<rbrace>"
-  unfolding vcpu_switch_def by (rule hoare_pre) wpsimp+
 
 lemma set_vcpu_etcbs_of[wp]:
   "set_vcpu ptr vcpu \<lbrace>\<lambda>s. P (etcbs_of s)\<rbrace>"
@@ -55,8 +36,9 @@ lemma set_vcpu_valid_queues [wp]:
   "\<lbrace>valid_queues\<rbrace> set_vcpu ptr vcpu \<lbrace>\<lambda>_. valid_queues\<rbrace>"
   by (rule valid_queues_lift; wp)
 
-crunch vcpu_switch
+crunch vcpu_switch, vcpu_flush
   for etcbs_of[wp]: "\<lambda>s. P (etcbs_of s)"
+  and scheduler_action[wp]: "\<lambda>s. P (scheduler_action s)"
   and ready_queues[wp]: "\<lambda>s. P (ready_queues s)"
   and cur_domain[wp]: "\<lambda>s. P (cur_domain s)"
   (wp: crunch_wps)
@@ -72,10 +54,6 @@ lemma set_vcpu_weak_valid_sched_action[wp]:
 lemma vcpu_switch_weak_valid_sched_action[wp]:
   "\<lbrace>weak_valid_sched_action\<rbrace> vcpu_switch v \<lbrace>\<lambda>_. weak_valid_sched_action\<rbrace>"
   by (rule weak_valid_sched_action_lift; wp)
-
-crunch set_vm_root
-  for pred_tcb_atP[wp]: "\<lambda>s. P (pred_tcb_at proj Q t s)"
-  (wp: crunch_wps simp: crunch_simps)
 
 lemma set_asid_pool_etcbs_of[wp]:
   "set_asid_pool ptr pool \<lbrace>\<lambda>s. P (etcbs_of s)\<rbrace>"
@@ -93,8 +71,7 @@ lemma set_asid_pool_valid_queues[wp]:
   by (wpsimp wp: valid_queues_lift)
 
 crunch set_asid_pool, set_vm_root, vcpu_flush
-  for scheduler_action[wp]: "\<lambda>s. P (scheduler_action s)"
-  and cur_domain[wp]: "\<lambda>s. P (cur_domain s)"
+  for cur_domain[wp]: "\<lambda>s. P (cur_domain s)"
   and ready_queues[wp]: "\<lambda>s. P (ready_queues s)"
 
 lemma set_asid_pool_weak_valid_sched_action[wp]:
@@ -116,13 +93,14 @@ lemma set_vcpu_valid_sched_action'[wp]:
              wp: hoare_vcg_imp_lift' hoare_vcg_all_lift | wps)+
 
 crunch
-  switch_to_idle_thread, switch_to_thread, set_vm_root, arch_get_sanitise_register_info,
+  switch_to_idle_thread, switch_to_thread, vcpu_restore, set_vm_root, arch_get_sanitise_register_info,
   arch_post_modify_registers, arch_prepare_next_domain
   for valid_queues [wp, DetSchedSchedule_AI_assms]: valid_queues
   (simp: crunch_simps wp: crunch_wps ignore: tcb_sched_action)
 
 crunch
-  switch_to_idle_thread, switch_to_thread, set_vm_root, arch_get_sanitise_register_info, arch_post_modify_registers
+  switch_to_idle_thread, switch_to_thread, vcpu_disable, vcpu_restore, vcpu_save, set_vm_root,
+  arch_get_sanitise_register_info, arch_post_modify_registers
   for weak_valid_sched_action [wp, DetSchedSchedule_AI_assms]: weak_valid_sched_action
   (simp: crunch_simps wp: crunch_wps)
 
@@ -136,7 +114,7 @@ lemma vcpu_switch_valid_sched_action[wp]:
   unfolding valid_sched_action_def is_activatable_def st_tcb_at_kh_simp
   by (rule hoare_lift_Pf[where f=cur_thread]; wpsimp wp: hoare_vcg_imp_lift switch_in_cur_domain_lift)
 
-lemma switch_to_idle_thread_ct_not_in_q [wp, DetSchedSchedule_AI_assms]:
+lemma switch_to_idle_thread_ct_not_in_q[wp, DetSchedSchedule_AI_assms]:
   "\<lbrace>valid_queues and valid_idle\<rbrace> switch_to_idle_thread \<lbrace>\<lambda>_. ct_not_in_q\<rbrace>"
   unfolding switch_to_idle_thread_def arch_switch_to_idle_thread_def
   apply (wpsimp | wps)+
@@ -164,7 +142,7 @@ crunch set_vm_root
                                                    (scheduler_action s) (cur_domain s) (etcbs_of s)"
   (wp: crunch_wps simp: crunch_simps ignore: set_asid_pool)
 
-lemma switch_to_idle_thread_ct_in_cur_domain [wp, DetSchedSchedule_AI_assms]:
+lemma switch_to_idle_thread_ct_in_cur_domain[wp, DetSchedSchedule_AI_assms]:
   "\<lbrace>\<top>\<rbrace> switch_to_idle_thread \<lbrace>\<lambda>_. ct_in_cur_domain\<rbrace>"
   unfolding switch_to_idle_thread_def arch_switch_to_idle_thread_def
   by (wpsimp wp: hoare_vcg_imp_lift' hoare_vcg_disj_lift | simp add: ct_in_cur_domain_def | wps)+
@@ -212,10 +190,6 @@ crunch
   for valid_sched[wp, DetSchedSchedule_AI_assms]: valid_sched
   (simp: crunch_simps wp: crunch_wps)
 
-crunch set_vm_root
-  for exst[wp]: "\<lambda>s. P (exst s)"
-  (wp: crunch_wps whenE_wp simp: crunch_simps)
-
 lemma arch_thread_set_ct_in_cur_domain_2[wp]:
   "arch_thread_set f tptr \<lbrace>\<lambda>s. ct_in_cur_domain_2 thread (idle_thread s) (scheduler_action s) (cur_domain s) (etcbs_of s)\<rbrace>"
   apply (simp add: arch_thread_set_def set_object_def get_object_def)
@@ -229,41 +203,10 @@ crunch set_asid_pool
   for valid_blocked[wp]: valid_blocked
   (wp: valid_blocked_lift)
 
-crunch set_vm_root
-  for valid_blocked[wp]: valid_blocked
-  (simp: crunch_simps)
-
 lemma set_asid_pool_ct_in_q[wp]:
   "set_asid_pool ptr pool \<lbrace>ct_in_q\<rbrace>"
   unfolding ct_in_q_def
   by (wpsimp wp: hoare_vcg_imp_lift' | wps)+
-
-crunch set_vm_root
-  for ct_in_q[wp]: ct_in_q
-  (simp: crunch_simps)
-
-crunch switch_to_thread
-  for etcb_at[wp, DetSchedSchedule_AI_assms]: "etcb_at P t"
-  (wp: crunch_wps)
-
-crunch
-  arch_switch_to_idle_thread
-  for valid_idle[wp, DetSchedSchedule_AI_assms]: "valid_idle"
-  (wp: crunch_wps simp: crunch_simps)
-
-crunch arch_switch_to_idle_thread, arch_prepare_next_domain
-  for etcb_at[wp, DetSchedSchedule_AI_assms]: "etcb_at P t"
-
-crunch
-  arch_prepare_next_domain, arch_prepare_set_domain
-  for scheduler_action[wp, DetSchedSchedule_AI_assms]: "\<lambda>s. P (scheduler_action s)"
-  (simp: Let_def)
-
-crunch vcpu_flush
-  for typ_at[wp]: "\<lambda>s. P (typ_at T p s)"
-  (wp: crunch_wps)
-
-lemmas vcpu_flush_typ_ats [wp] = abs_typ_at_lifts[OF vcpu_flush_typ_at]
 
 crunch vcpu_switch, arch_prepare_next_domain
   for ready_queues[wp, DetSchedSchedule_AI_assms]: "\<lambda>s. P (ready_queues s)"
@@ -292,6 +235,11 @@ lemma arch_prepare_next_domain_ct_in_q[wp, DetSchedSchedule_AI_assms]:
   unfolding ct_in_q_def
   by (wp_pre, wps, wpsimp+)
 
+crunch set_vm_root
+  for valid_blocked[wp]: valid_blocked
+  and ct_in_q[wp]: ct_in_q
+  (wp: valid_blocked_lift hoare_vcg_imp_lift' simp: crunch_simps)
+
 lemma set_vm_root_valid_blocked_ct_in_q [wp]:
   "\<lbrace>valid_blocked and ct_in_q\<rbrace> set_vm_root p \<lbrace>\<lambda>_. valid_blocked and ct_in_q\<rbrace>"
   by wpsimp
@@ -301,11 +249,22 @@ crunch lazy_fpu_restore
   and ct_in_q[wp]: ct_in_q
   (wp: crunch_wps)
 
-lemma arch_switch_to_thread_valid_blocked [wp, DetSchedSchedule_AI_assms]:
+lemma arch_switch_to_thread_valid_blocked[wp, DetSchedSchedule_AI_assms]:
   "\<lbrace>valid_blocked and ct_in_q\<rbrace> arch_switch_to_thread thread \<lbrace>\<lambda>_. valid_blocked and ct_in_q\<rbrace>"
   by (wpsimp simp: arch_switch_to_thread_def)
 
-lemma switch_to_idle_thread_ct_not_queued [wp, DetSchedSchedule_AI_assms]:
+crunch arch_switch_to_thread, arch_switch_to_idle_thread, arch_prepare_next_domain
+  for etcb_at[wp, DetSchedSchedule_AI_assms]: "etcb_at P t"
+
+crunch arch_switch_to_idle_thread
+  for valid_idle[wp, DetSchedSchedule_AI_assms]: "valid_idle"
+  (wp: crunch_wps simp: crunch_simps)
+
+crunch arch_prepare_next_domain, arch_prepare_set_domain
+  for scheduler_action[wp, DetSchedSchedule_AI_assms]: "\<lambda>s. P (scheduler_action s)"
+  (simp: Let_def)
+
+lemma switch_to_idle_thread_ct_not_queued[wp, DetSchedSchedule_AI_assms]:
   "\<lbrace>valid_queues and valid_idle\<rbrace>
      switch_to_idle_thread
    \<lbrace>\<lambda>rv s. not_queued (cur_thread s) s\<rbrace>"
@@ -352,14 +311,14 @@ lemma astit_st_tcb_at[wp]:
   apply (simp add: arch_switch_to_idle_thread_def)
   by (wpsimp)
 
-lemma stit_activatable' [DetSchedSchedule_AI_assms]:
+lemma stit_activatable'[DetSchedSchedule_AI_assms]:
   "\<lbrace>valid_idle\<rbrace> switch_to_idle_thread \<lbrace>\<lambda>rv . ct_in_state activatable\<rbrace>"
   apply (simp add: switch_to_idle_thread_def ct_in_state_def do_machine_op_def split_def)
   apply wpsimp
   apply (clarsimp simp: valid_idle_def ct_in_state_def pred_tcb_at_def obj_at_def)
   done
 
-lemma switch_to_idle_thread_cur_thread_idle_thread [wp, DetSchedSchedule_AI_assms]:
+lemma switch_to_idle_thread_cur_thread_idle_thread[wp, DetSchedSchedule_AI_assms]:
   "\<lbrace>\<top>\<rbrace> switch_to_idle_thread \<lbrace>\<lambda>_ s. cur_thread s = idle_thread s\<rbrace>"
   by (wp | simp add:switch_to_idle_thread_def arch_switch_to_idle_thread_def)+
 
@@ -387,14 +346,6 @@ crunch
   for ct_not_in_q[wp, DetSchedSchedule_AI_assms]: ct_not_in_q
   (wp: crunch_wps hoare_drop_imps unless_wp select_inv mapM_wp
        subset_refl if_fun_split simp: crunch_simps ignore: tcb_sched_action)
-
-crunch arch_thread_set
-  for etcbs_of[wp]: "\<lambda>s. P (etcbs_of s)"
-  (wp: set_object_wp)
-
-lemma arch_thread_set_valid_sched[wp]:
-  "arch_thread_set f p \<lbrace>valid_sched\<rbrace>"
-  by (wpsimp wp: valid_sched_lift arch_thread_set_pred_tcb_at)
 
 crunch
   arch_finalise_cap, prepare_thread_delete
@@ -523,6 +474,12 @@ crunch arch_switch_to_thread, handle_spurious_irq
   and valid_idle[wp, DetSchedSchedule_AI_assms]: valid_idle
   and cur_domain[wp, DetSchedSchedule_AI_assms]: "\<lambda>s. P (cur_domain s)"
   and etcbs_of[wp, DetSchedSchedule_AI_assms]: "\<lambda>s. P (etcbs_of s)"
+
+crunch prepare_thread_delete, arch_post_cap_deletion, arch_finalise_cap
+  for cur_thread[wp, DetSchedSchedule_AI_assms]: "\<lambda>s. P (cur_thread s)"
+  and cur_domain[wp, DetSchedSchedule_AI_assms]: "\<lambda>s. P (cur_domain s)"
+  and etcbs_of[wp, DetSchedSchedule_AI_assms]: "\<lambda>s. P (etcbs_of s)"
+  (wp: crunch_wps simp: crunch_simps)
 
 end
 
